co and co_of removed

theories/Interaction_Between_Lts/Examples_of_Interactions/ForwarderConstruction.v
@@ -36,7 +36,7 @@ From Must Require Import MultisetHelper gLts Bisimulation Lts_OBA Lts_FW Lts_OBA
 
 (**************************************** Forwarder LTS *************************************)
 
-Definition fw_inter `{ExtAction A} μ2 μ1 := dual μ1 μ2 /\ non_blocking μ1.
+Definition fw_inter `{ExtAction A} μ2 μ1 := dual μ2 μ1 /\ non_blocking μ1.
 
 #[global] Program Instance FW_gLts {P A : Type} `{H : ExtAction A} (M: gLts P A) 
   `{@Prop_of_Inter P (mb A) A fw_inter H M MbgLts}
@@ -160,9 +160,9 @@ Notation "p ⟶≐[ μ ] q" := (lts_fw_sc p (ActExt μ) q) (at level 90, format 
 
 (* Properties on our FW Equivalence, to assert it is a simulation. *)
 
-Lemma fw_eq_blocking_action_simulation `{gLtsOba P A} {p q mp mq μ q'} :
-  p ▷ mp ≐ q ▷ mq -> blocking μ  -> q ⟶[μ] q'
-    -> exists p', p ⟶[μ] p' /\ p' ▷ mp ≐ q' ▷ mq.
+Lemma fw_eq_blocking_action_simulation `{gLtsOba P A} {p q mp mq β q'} :
+  p ▷ mp ≐ q ▷ mq -> blocking β  -> q ⟶[β] q'
+    -> exists p', p ⟶[β] p' /\ p' ▷ mp ≐ q' ▷ mq.
 Proof.
   intros heq not_nb hlq. 
   edestruct (lts_oba_mo_strip p) as (p0 & hwp).
@@ -173,7 +173,7 @@ Proof.
   edestruct (strip_delay_inp4 not_nb hlq hwq') as (q2 & hwq2 & hlq2).
   assert (q0 ⋍ q2) by (eapply strip_m_deter; eauto).
   destruct hlq2 as (r & hlr & heqr).
-  edestruct (eq_spec p0 r (ActExt $ μ)) as (p0' & hlp0' & heqp0').
+  edestruct (eq_spec p0 r (ActExt $ β)) as (p0' & hlp0' & heqp0').
   exists q2. split; eauto. transitivity q0; eauto.
   edestruct (strip_retract_act hwp hlp0' ) as (p' & wp' & p1 & hwp' & heqp').
   exists p'. split. eassumption.
@@ -201,9 +201,9 @@ Qed.
 Lemma lts_fw_eq_spec_left_blocking_action `{
    M : @gLtsObaFB P A H gLtsP gLtsEqP gLtsObaP}
    `{@Prop_of_Inter P (mb A) A fw_inter H gLtsP MbgLts}
-   p q q' mp mq μ :
-   p ▷ mp ≐ q ▷ mq -> blocking μ -> q ⟶[μ] q'
-    -> p ▷ mp ⟶≐[μ] q' ▷ mq.
+   p q q' mp mq β :
+   p ▷ mp ≐ q ▷ mq -> blocking β -> q ⟶[β] q'
+    -> p ▷ mp ⟶≐[β] q' ▷ mq.
 Proof.
   intros not_nb heq l.
   edestruct (fw_eq_blocking_action_simulation not_nb heq l) as (p' & hl' & heq').
@@ -468,7 +468,7 @@ Lemma lts_fw_eq_spec_right_blocking_action `{
   M : @gLtsObaFB P A H gLtsP gLtsEqP gLtsObaP}
   `{@Prop_of_Inter P (mb A) A fw_inter H gLtsP MbgLts}
    p q mp mq η μ:
-  non_blocking η -> dual η μ -> p ▷ mp ≐ q ▷ mq 
+  non_blocking η -> dual μ η -> p ▷ mp ≐ q ▷ mq 
     -> p ▷ mp ⟶≐[μ] q ▷ {[+ η +]} ⊎ mq.
 Proof.
   intros nb duo heq.
@@ -485,8 +485,8 @@ Qed.
 Lemma lts_fw_com_eq_spec `{
   M : @gLtsObaFB P A H gLtsP gLtsEqP gLtsObaP}
   `{@Prop_of_Inter P (mb A) A fw_inter H gLtsP MbgLts}
-  p q q' mp mq μ η:
-  blocking μ -> dual η μ -> non_blocking η -> p ▷ mp ≐ q ▷ {[+ η +]} ⊎ mq -> q ⟶[μ] q' 
+  p q q' mp mq β η:
+  blocking β -> dual β η -> non_blocking η -> p ▷ mp ≐ q ▷ {[+ η +]} ⊎ mq -> q ⟶[β] q' 
     -> p ▷ mp ⟶≐ q' ▷ mq.
 Proof.
   intros not_nb duo nb' heq hl.
@@ -500,7 +500,7 @@ Proof.
     by (now rewrite heqm; multiset_solver).
   eapply gmultiset_elem_of_disj_union in mem as [hleft | hright].
   - eapply lts_oba_mo_spec_bis2 in hleft as (p1 & nb & hl1).
-    assert (neq : μ ≠ η). eapply BlockingAction_are_not_non_blocking; eauto.
+    assert (neq : β ≠ η). eapply BlockingAction_are_not_non_blocking; eauto.
     edestruct (lts_oba_non_blocking_action_confluence nb neq hl1 hl') as (p2 & hlp1 & hlp').
     edestruct (lts_oba_fb_feedback nb duo hl1 hlp1) as (p3 & hlp & heqp3).
     exists (p3, mp). split.
@@ -645,7 +645,7 @@ Next Obligation.
 Qed.
 Next Obligation.
 intros ? ? ? ? ? ? ? ? ? ? ? ? ? nb Hstep_nb Hstep. destruct p as (p, mp), q as (q, mq), r as (r, mr).
-  inversion Hstep_nb (* as [a b c d e f| a b c d e f| a b c d e f] *) ; inversion Hstep; subst.
+  inversion Hstep_nb; inversion Hstep; subst.
   - destruct (lts_oba_non_blocking_action_delay nb l l0) as (t & hlt0 & (r0 & hlr0 & heqr0)).
     exists (t, mr). split; simpl in *. eauto with mdb.
     exists (r0, mr). split. simpl in *. eauto with mdb.
@@ -921,7 +921,7 @@ Qed.
 
 Definition lts_fw_not_non_blocking_action_set `{FiniteImagegLts P A} 
   (p : P) (m : mb A) μ :=
-  if (decide (dual (co μ) μ /\ non_blocking (co μ))) 
+  if (decide (dual μ (co μ) /\ non_blocking (co μ))) 
   then (p, {[+ (co μ) +]} ⊎ m) :: map (fun p => (proj1_sig p, m)) (enum $ dsig (lts_step p (ActExt $ μ)))
   else map (fun p => (proj1_sig p, m)) (enum $ dsig (lts_step p (ActExt $ μ))).
 
@@ -1039,23 +1039,23 @@ Qed.
 
 Lemma lts_fw_input_set_spec1 `{@FiniteImagegLts P A H gLtsP}
   `{@Prop_of_Inter P (mb A) A fw_inter H gLtsP MbgLts}
-  p1 m1 p2 m2 μ :
-  (p1, m1) ⟶[μ] (p2, m2) -> blocking μ -> 
-    (p2, m2) ∈ lts_fw_not_non_blocking_action_set p1 m1 μ.
+  p1 m1 p2 m2 β :
+  (p1, m1) ⟶[β] (p2, m2) -> blocking β -> 
+    (p2, m2) ∈ lts_fw_not_non_blocking_action_set p1 m1 β.
 Proof.
   intros l not_nb.
   inversion l; subst.
   + unfold lts_fw_not_non_blocking_action_set.
-    destruct (decide (dual (co μ) μ /\ non_blocking (co μ))) as [(duo & nb) | case2].
+    destruct (decide (dual β (co β) /\ non_blocking (co β))) as [(duo & nb) | case2].
     - right. eapply elem_of_list_fmap.
       exists (dexist p2 l0). split. reflexivity. eapply elem_of_enum.
     - eapply elem_of_list_fmap.
       exists (dexist p2 l0). split. reflexivity. eapply elem_of_enum.
-  + eapply (blocking_action_in_ms m1 μ m2) in not_nb as (eq & duo & nb); eauto; subst.
+  + eapply (blocking_action_in_ms m1 β m2) in not_nb as (eq & duo & nb); eauto; subst.
     unfold lts_fw_not_non_blocking_action_set.
-    destruct (decide (dual (co μ) μ /\ non_blocking (co μ))) as [toto | impossible].
+    destruct (decide (dual β (co β) /\ non_blocking (co β))) as [toto | impossible].
     ++ left.
-    ++ assert (dual (co μ) μ ∧ non_blocking (co μ)); eauto. contradiction.
+    ++ assert (dual β (co β) ∧ non_blocking (co β)); eauto. contradiction.
 Qed. 
 
 Lemma lts_fw_non_blocking_action_set_spec1 `{@FiniteImagegLts P A H gLtsP}
