theories/Testing_Pre_orders/Must/Lift.v
@@ -69,7 +69,7 @@ Proof.
       destruct le as (e' & hle' & heqe').
       eapply nh, (outcome_preserved_by_eq e' e2); eauto.
       eapply outcome_preserved_by_lts_non_blocking_action; eauto.
-    + destruct (exists_duo_nb η) as (μ & duo).
+    + destruct (exists_dual η) as (μ & duo). symmetry in duo.
       destruct (lts_oba_fw_forward p2 η μ) as (p'2 & Hyp).
       destruct (Hyp nb duo) as (Tr1 & Tr2). 
       destruct le as (e'1 & Tr & eq).
@@ -321,10 +321,10 @@ Proof.
     -- dependent induction hm; subst. 
       + eapply m_now. eapply outcome_preserved_by_lts_non_blocking_action; eassumption.
       + assert (non_blocking η) as nb. eauto.
-        edestruct exists_duo_nb as (μ & duo). 
+        edestruct (exists_dual η) as (μ & duo). symmetry in duo.
         eapply com; eauto.
-        eapply ParRight. assert (¬ non_blocking μ) as not_nb.
-        eapply dual_blocks; eauto.
+        eapply ParRight. assert (blocking μ) as not_nb.
+        { eapply dual_blocks; eauto. }
         eapply lts_multiset_add; eauto.
     -- replace ({[+ η +]} ⊎ m ⊎ m2) with (m ⊎ ({[+ η +]} ⊎ m2)) by multiset_solver.
        eapply IHhwo. eassumption.
@@ -482,8 +482,10 @@ Proof.
                  multiset_solver. rewrite<- eq''. eauto. rewrite H11.
                  eapply mo_stripped_equiv; eauto. symmetry; eauto.
             ++++ eapply blocking_action_in_ms in not_nb1 as (eq & duo' & nb'); subst ; eauto.
-                 assert (non_blocking μ2). eapply nb_not_nb; eauto.
-                 contradiction.
+                 assert (non_blocking μ2).
+                 assert (μ2 = co μ1). 
+                 { eapply unique_nb in duo. eauto. } 
+                 subst. eauto. contradiction.
 Qed.
 
 Lemma must_fw_to_must `{
@@ -530,7 +532,7 @@ Proof.
                     eapply lts_oba_mo_spec_bis2 in mem as (e2 & nb' & l'2).
                     assert (neq : μ2 ≠ μ1). eapply BlockingAction_are_not_non_blocking; eauto.
                     edestruct (lts_oba_non_blocking_action_confluence nb' neq l'2 l0) as (e3 & l3 & l4).
-                    assert (dual μ1 μ2) as duo. symmetry; eauto.
+                    assert (dual μ2 μ1) as duo. { symmetry. eauto. }
                     destruct (lts_oba_fb_feedback nb' duo l'2 l3) as (e4 & l6 & _).
                     exists (p0 ▷ e4). eapply ParRight; eauto.
           +++ inversion l1; subst.
@@ -539,8 +541,8 @@ Proof.
                    exists (p0, r).
                    eapply ParSync; eauto.
               ++++ eapply blocking_action_in_ms in n0 as (eq' & duo' & nb'); eauto; subst.
-                   assert (non_blocking μ2) as nb''.
-                   eapply nb_not_nb. eauto. exact duo'. eauto. contradiction.
+                   assert (μ2 = co μ1). { eapply unique_nb;eauto. }
+                   subst. contradiction.
     - intros p' l. eapply H8; eauto with mdb. eapply ParLeft; eauto.
     - intros p' e' μ1 μ2 duo l1 l2. eapply H6; eauto with mdb. eapply ParLeft; eauto.
 Qed.
